\documentclass[11pt]{article}

\usepackage[shortlabels]{enumitem}
\usepackage[margin=1in,headheight=15pt]{geometry}   % Adjusted headheight
\usepackage{amsmath}
\usepackage{fancyhdr}
\usepackage{graphicx}
\usepackage{cancel}
\usepackage{amsfonts}

% Set up fancy header/footer
\pagestyle{fancy}
\fancyhead[LO,L]{Jimmy Chen}
\fancyhead[CO,C]{CSCI 2500 - Computer Organization}
\fancyhead[RO,R]{November 13, 2023}
\fancyfoot[LO,L]{}
\fancyfoot[CO,C]{\thepage}
\fancyfoot[RO,R]{}
\renewcommand{\headrulewidth}{0.4pt}
\renewcommand{\footrulewidth}{0.4pt}

\begin{document}
\section{Homework 3}

% BOOLEAN ALGEBRA QUESTIONS
\subsection{Boolean Algebra}
\begin{enumerate}
    \item Simplify the following expressions using Boolean algebraic laws. Give each step of your simplification and denote which laws youâ€™re using for each step. Do not skip or combine steps!
    \begin{enumerate}[(a)]
        % =========Question 1a=========
        \item  $A * (\overline{A}+B*B) + (\overline{B+A}) * (\overline{A} + B)$\\
        \textbf{Work:}
        \begin{center}
            $A * (\overline{A} + B) + (\overline{B + A}) * (\overline{A} + B)$ // Idempotent law\\
            $A * B + (\overline{B + A}) * (\overline{A} + B)$ // Redundancy law\\
            $A * B + \overline{B} * \overline{A} * (\overline{A} + B)$ // Demorgan's law\\
            \fbox{\begin{minipage}{15em}
                \begin{center}
                \textbf{Answer: $A * B + \overline{B} * \overline{A}$}
                \end{center}
            \end{minipage}}
        \end{center} 
        % =========Question 1b=========
        \item $\overline{C * B} + ( A * B * C) + \overline{A + B + \overline{B}}$\\
        \textbf{Work:}
        \begin{center}
            $\overline{C} + \overline{B} + (A * B * C) + \overline{A + C + \overline{B}}$ // Demorgan's law\\
            $\overline{C} + \overline{B} + (A * B * C) + \overline{A} * \overline{C} * B$ // Involution Law\\
            $\overline{C} + \overline{B} + A * B * C$ // Absorption Law\\
            $\overline{C} + \overline{B} + A * B$ // Absorption Law\\
            $\overline{C} + \overline{B} + A$ // Absorption Law\\
            \fbox{\begin{minipage}{15em}
                \begin{center}
                \textbf{Answer: $\overline{C} + \overline{B} + A$}
                \end{center}
            \end{minipage}}
        \end{center}
        % =========Question 1c=========
        \item $(A + B) * (\overline{A} + C) * (\overline{C} + B)$ \\
        \textbf{Work:}
        \begin{center}
            $(\overline{A} + C) * (\overline{C} + B) * A + (\overline{A} + C) * (\overline{C} + B) * B$ // Distributive Law\\
            $(\overline{C} + B) * A * \overline{A} + (\overline{C} + B) * A * C + (\overline{A} + C) * (\overline{C} + B) * B$ // Distributive Law\\
            $0 + (\overline{C} + B) * A * C + (\overline{A} + C) * (\overline{C} + B) * B$ // Complement Law\\
            $(\overline{C} + B) * A * C + (\overline{A} + C) * (\overline{C} + B) * B$ // Identity Law\\
            $A * A * \overline{C} + A * C * B + (\overline{A} + C) * (\overline{C} + B) * B$ // Distributive Law\\
            $0 + A * C * B + (\overline{A} + C) * (\overline{C} + B) * B$ // Complement Law\\
            $A * C * B + (\overline{A} + C) * (\overline{C} + B) * B$ // Identity Law\\
            $A * C * B + B * \overline{A} * \overline{C} + B * \overline{A} * B + (\overline{C} + B) * B * C$ // Distributive Law\\
            $A * C * B + B * \overline{A} + (\overline{C} + B) * B * C$ // Absorption Law\\
            $B * (A * C + \overline{A}) + (\overline{C} + B) * B * C$ // Distributive Law\\
            $B * (C + \overline{A}) + (\overline{C} + B) * B * C$ // Absorption Law\\
            $B * C + B * \overline{A} + (\overline{C} + B) * B * C$ // Distributive Law\\
            $B * C + B * \overline{A}$ // Absorption Law\\
            \fbox{\begin{minipage}{15em}
                \begin{center}
                \textbf{Answer: $B * C + B * \overline{A}$}
                \end{center}
            \end{minipage}}
        \end{center}
    \end{enumerate}
    
    \item Find all solutions of the following Boolean equations without using the truth tables:
    \begin{enumerate}[(a)]
        \item $(\overline{A} + C) * (\overline{B} + D + A) * (D + A * \overline{C}) * (\overline{D} + A) = 1$\\
        \textbf{Work:}
        \item $(((\overline{K} * L * N) * (L * M)) + ((\overline{K} + L + N) * (K * \overline{L} * \overline{M}))) * (\overline{K} + \overline{N}) = 1$\\
        \textbf{Work:}
    \end{enumerate}

    \item Simplify the following expression by first constructing a truth table, using that truth table to
    construct a K-map, and then using that K-map to simplify.\\
    $Q = \overline{X} * \overline{Y} * Z + X * Y * \overline{Z} + \overline{X} + Y * \overline{Z} + X * \overline{Y} * \overline{Z}$\\
    \textbf{Work:}
\end{enumerate}
\subsection{Logical Circuits}
\begin{enumerate}
    \item Convert the following truth table into its sum of products representation:
\end{enumerate}
\end{document}
